src/tls/MAC.fst
@@ -2,6 +2,7 @@
 
 open FStar.Heap
 open FStar.HyperHeap
+open FStar.HyperStack
 open FStar.Seq
 open FStar.SeqProperties // for e.g. found
 
@@ -25,7 +26,7 @@ type tag (i:id) = lbytes (macSize (alg i))
 type keyrepr (i:id) = bytes
 
 
-type fresh_subregion rg parent h0 h1 = fresh_region rg h0 h1 /\ extends rg parent
+type fresh_subregion rg parent h0 h1 = stronger_fresh_region rg h0 h1 /\ extends rg parent
 
 // We keep the tag in case we later want to enforce tag authentication
 abstract type entry (i:id) (good: bytes -> Type) = 
@@ -33,10 +34,15 @@ abstract type entry (i:id) (good: bytes -> Type) =
 
 // readers and writers share the same private state: a log of MACed messages
 // TODO make it abstract
+(*
+ * AR: two changes: region is of type rgn.
+ * log is a hyperstack ref with refinement capturing its rid.
+ *)
 noeq type key (i:id) (good: bytes -> Type) = 
-  | Key: #region : rid -> // intuitively, the writer's region
+  | Key: #region : rgn -> // intuitively, the writer's region
          kv      : keyrepr i ->
-         log     : rref region (seq (entry i good)) -> key i good
+	 log     : ref (seq (entry i good)){log.id = region}
+	 -> key i good
 
 val region: #i:id -> #good:(bytes -> Type) -> k:key i good -> GTot rid
 val keyval: #i:id -> #good:(bytes -> Type) -> k:key i good -> GTot (keyrepr i)
@@ -44,28 +50,27 @@ val keyval: #i:id -> #good:(bytes -> Type) -> k:key i good -> GTot (keyrepr i)
 let region #i #good (k:key i good) = k.region
 let keyval #i #good (k:key i good) = k.kv 
 
-val gen: i:id -> good: (bytes -> Type) -> parent: rid -> ST(key i good)
-  (requires (fun _ -> True))
-  (ensures (fun h0 k h1 ->  
-    modifies Set.empty h0 h1 /\
-    fresh_subregion (region #i #good k) parent h0 h1 )) 
-
-val coerce: i:id -> good: (bytes -> Type) -> parent: rid -> kv:keyrepr i -> ST(key i good)
-  (requires (fun _ -> ~(authId i)))
-  (ensures (fun h0 k h1 ->  
-    modifies Set.empty h0 h1 /\
-    fresh_subregion (region #i #good k) parent h0 h1 )) 
-
-val leak: #i:id -> #good: (bytes -> Type) -> k:key i good {~(authId i)} -> Tot (kv:keyrepr i { kv = keyval k })
-
 // todo: mark it as private
 private let gen0 i good parent kv = 
   let region = new_region parent in 
   let log = ralloc region Seq.createEmpty in 
   Key #i #good #region kv log
 
+val gen: i:id -> good: (bytes -> Type) -> parent: rgn -> ST(key i good)
+  (requires (fun _ -> True))
+  (ensures (fun h0 k h1 ->  
+    modifies Set.empty h0 h1 /\
+    fresh_subregion (region #i #good k) parent h0 h1 )) 
 let gen    i good parent    = gen0 i good parent (CoreCrypto.random (macKeySize (alg i)))
+
+val coerce: i:id -> good: (bytes -> Type) -> parent: rgn -> kv:keyrepr i -> ST(key i good)
+  (requires (fun _ -> ~(authId i)))
+  (ensures (fun h0 k h1 ->  
+    modifies Set.empty h0 h1 /\
+    fresh_subregion (region #i #good k) parent h0 h1 )) 
 let coerce i good parent kv = gen0 i good parent kv
+
+val leak: #i:id -> #good: (bytes -> Type) -> k:key i good {~(authId i)} -> Tot (kv:keyrepr i { kv = keyval k })
 let leak   #i #good k = k.kv
 
 val mac: #i:id -> #good:(bytes -> Type) -> k:key i good -> p:bytes { authId i ==> good p } -> ST(tag i) 
@@ -78,11 +83,15 @@ val mac: #i:id -> #good:(bytes -> Type) -> k:key i good -> p:bytes { authId i ==
 
 
 // We log every authenticated texts, with their index and resulting tag
+(*
+ * AR: had to add a recall to satisfy the precondition of k.log write.
+ *)
 let mac #i #good k p =
   assume (HashMAC.is_tls_mac (alg i));
   let p : p:bytes { authId i ==> good p } = p in
   let t = HashMAC.tls_mac (alg i) k.kv p in
   let e : entry i good = Entry t p in
+  recall k.log;
   k.log := snoc !k.log e;
   t
 
